refactoring and renaming

Source/Core/node.bpl
@@ -77,8 +77,12 @@ axiom {:ctor "Node"} (forall<T> f: [One Loc]Node T, u: Option Loc, v: Option Loc
     (Avoiding(f, u, Some(p), x) && Some(p) != x && Avoiding(f, q->next, v, Some(p)) && Avoiding(f, q->next, v, x))
 );
 
-function {:inline} ListInDomain<V>(start: Option Loc, nodes: Map (One Loc) (Node V)): bool {
-  (forall x: Loc:: BetweenSet(nodes->val, start, None())[x] ==> Set_Contains(nodes->dom, One(x)))
+function {:inline} InDomain<V>(nodes: Map (One Loc) (Node V), start: Option Loc): bool {
+  (forall x: Loc:: Between(nodes->val, start, Some(x), None()) ==> Set_Contains(nodes->dom, One(x)))
+}
+
+function {:inline} Reachable<V>(nodes: Map (One Loc) (Node V), start: Option Loc, elem: Option Loc): bool {
+  Between(nodes->val, start, elem, elem)
 }
 
 function StackAbs<V>(start: Option Loc, nodes: Map (One Loc) (Node V)): Vec V;
@@ -88,20 +92,9 @@ if start == None() then
   (var n := Map_At(nodes, One(start->t)); Vec_Append(StackAbs(n->next, nodes), n->val))
 }
 
-pure procedure StackAbsCompute<V>(start: Option Loc, nodes: Map (One Loc) (Node V), nodes': Map (One Loc) (Node V)) returns (absStack: Vec V);
-requires Set_IsSubset(nodes->dom, nodes'->dom);
-requires MapIte(nodes->dom, nodes->val, MapConst(Default())) ==
-         MapIte(nodes->dom, nodes'->val, MapConst(Default()));
-requires Between(nodes->val, start, start, None());
-requires ListInDomain(start, nodes);
-ensures absStack == StackAbsDef(start, nodes);
-ensures absStack == StackAbsDef(start, nodes');
-free ensures absStack == StackAbs(start, nodes);
-free ensures absStack == StackAbs(start, nodes');
-
 pure procedure StackAbsLemma<V>(start: Option Loc, nodes: Map (One Loc) (Node V));
 requires Between(nodes->val, start, start, None());
-requires ListInDomain(start, nodes);
+requires InDomain(nodes, start);
 ensures StackAbs(start, nodes) == StackAbsDef(start, nodes);
 
 pure procedure StackFrameLemma<V>(start: Option Loc, nodes: Map (One Loc) (Node V), nodes': Map (One Loc) (Node V));
@@ -109,5 +102,5 @@ requires Set_IsSubset(nodes->dom, nodes'->dom);
 requires MapIte(nodes->dom, nodes->val, MapConst(Default())) ==
          MapIte(nodes->dom, nodes'->val, MapConst(Default()));
 requires Between(nodes->val, start, start, None());
-requires ListInDomain(start, nodes);
+requires InDomain(nodes, start);
 ensures StackAbs(start, nodes) == StackAbs(start, nodes');
